examples/low-level/crypto/Crypto.Symmetric.Poly1305.Spec.fst
@@ -22,13 +22,19 @@ module U8  = FStar.UInt8
 module U32 = FStar.UInt32
 module U64 = FStar.UInt64
 
-// missing overloading...
-//inline let op_Array_Access (#a:Type) (s:Seq.seq a) n = Seq.index s n
+#reset-options "--initial_fuel 4 --max_fuel 4"
 
-let p_1305 : nat = pow2 130 - 5  // prime (do we prove it? use it?)
+// prime (do we prove it? use it?)
+let p_1305: p:nat{pow2 128 < p} = 
+  cut (pow2 3 = 8); 
+  Math.Lib.pow2_increases_lemma 130 129;
+  Math.Lib.pow2_increases_lemma 129 128; 
+  pow2_increases_lemma 130 3; 
+  pow2 130 - 5
 
-type elem = n:nat{n < p_1305}    // elements of the field Z / p_1305 Z
+#reset-options
 
+type elem = n:nat{n < p_1305} // elements of the field Z / p_1305 Z
 
 type word = b: seq byte {Seq.length b <= 16} 
 type word_16 = b:seq byte {Seq.length b = 16} 
@@ -44,36 +50,36 @@ val field_add: elem -> elem -> Tot elem
 let field_add a b = (a + b) % p_1305 
 val field_mul: elem -> elem -> Tot elem
 let field_mul a b = (a * b) % p_1305 
+
 (* Infix operators for readability *)
 let op_Plus_At = field_add
 let op_Star_At = field_mul
 
 (* Little endian integer value of a sequence of bytes *)
-let rec little_endian (b:word) : Tot (n:nat) (decreases (Seq.length b))
-  = if Seq.length b = 0 then 0
-    else U8.v (Seq.index b 0) +
-	 pow2 8 * little_endian (Seq.slice b 1 (Seq.length b))
+let rec little_endian (b:word) : Tot (n:nat) (decreases (Seq.length b)) =
+  if Seq.length b = 0 then 0
+  else U8.v (Seq.index b 0) +
+       pow2 8 * little_endian (Seq.slice b 1 (Seq.length b))
 
 val lemma_euclidian_division: a:nat -> b:nat -> Lemma
   (requires (a < pow2 8))
-  (ensures  (a + pow2 8 * b < pow2 8 * (b+1)))
+  (ensures  (a + pow2 8 * b < pow2 8 * (b + 1)))
 let lemma_euclidian_division a b = ()
 
-val lemma_factorise: a:nat -> b:nat -> Lemma
-  (requires (True))
-  (ensures  (a + a * b = a * (b + 1)))
+val lemma_factorise: a:nat -> b:nat -> Lemma (a + a * b = a * (b + 1))
 let lemma_factorise a b = ()
 
-//TMP#reset-options "--z3timeout 100"
+//#reset-options "--z3timeout 200
 #set-options "--lax" // OK, but long timeout
 
 val lemma_little_endian_is_bounded: b:word -> Lemma
-  (requires (True))
-  (ensures  (little_endian b < pow2 (8*(Seq.length b))))
+  (requires True)
+  (ensures  (little_endian b < pow2 (8 * Seq.length b)))
   (decreases (Seq.length b))
 let rec lemma_little_endian_is_bounded b =
   if Seq.length b = 0 then ()
-  else (
+  else
+    begin
     let s = Seq.slice b 1 (Seq.length b) in
     assert(Seq.length s = Seq.length b - 1);
     lemma_little_endian_is_bounded s;
@@ -85,7 +91,7 @@ let rec lemma_little_endian_is_bounded b =
     assert(little_endian b <= pow2 8 * pow2 (8 * (Seq.length b - 1)));
     Math.Lemmas.pow2_exp_1 8 (pow2 (8 * (Seq.length b - 1)));
     lemma_factorise 8 (Seq.length b - 1)
-  )
+    end
 
 #reset-options
 
@@ -99,74 +105,89 @@ let lemma_little_endian_lt_2_128 b =
   else Math.Lib.pow2_increases_lemma 128 (8 * Seq.length b)
 
 
-let encode_16 (w:word_16) : elem = pow2 128  +@  little_endian w 
-// not using the lemma below?
+(* * *********************************************)
+(* *            Encoding                         *)
+(* * *********************************************)
+
+let encode_16 (w:word_16) : elem = pow2 128 +@ little_endian w
+
+// a spec for encoding and padding, convenient for injectivity proof
+let pad_0 b l = Seq.append b (Seq.create l 0uy)
+
+val encode_pad: prefix:Seq.seq elem -> txt:Seq.seq UInt8.t -> GTot (Seq.seq elem) 
+  (decreases (Seq.length txt))
+let rec encode_pad prefix txt =
+  let l = Seq.length txt in
+  if l = 0 then prefix
+  else if l < 16 then
+    begin
+    let w = pad_0 txt (16 - l) in
+    SeqProperties.snoc prefix (encode_16 w)
+    end
+  else
+    begin
+    let w, txt = SeqProperties.split txt 16 in
+    let prefix = SeqProperties.snoc prefix (encode_16 w) in
+    encode_pad prefix txt
+    end
 
 let trunc_1305 (e:elem) = e % pow2 128
+
 
 (* * *********************************************)
 (* *          Encoding-related lemmas            *)
 (* * *********************************************)
 
-let lemma_little_endian_is_injective_0 (b:word{Seq.length b > 0}) : Lemma
-  (requires (True))
-  (ensures  (little_endian b = U8.v (Seq.index b 0) + pow2 8 * little_endian (Seq.slice b 1 (Seq.length b)) ))
-  = ()
+#reset-options "--initial_fuel 1 --max_fuel 1 --initial_ifuel 0 --max_ifuel 0"
 
-//TMP#reset-options "--initial_fuel 0 --max_fuel 0"
+val lemma_little_endian_is_injective_0: b:word{Seq.length b > 0} -> Lemma
+  (little_endian b =
+   U8.v (Seq.index b 0) + pow2 8 * little_endian (Seq.slice b 1 (Seq.length b)))
+let lemma_little_endian_is_injective_0 b = ()
 
-(* Lemma unknown to F*, should go into core libraries *)
-assume val lemma_modulo: a:nat -> b:nat -> c:pos -> Lemma
-  (requires (True))
-  (ensures   ((a + b * c) % c = a))
-
-let lemma_little_endian_is_injective_1 (b:pos) (q:nat) (r:nat) (q':nat) (r':nat) : Lemma
+val lemma_little_endian_is_injective_1: b:pos -> q:nat -> r:nat -> q':nat -> r':nat -> Lemma
   (requires (r < b /\ r' < b /\ r + b * q = r' + b * q'))
   (ensures  (r = r' /\ q = q'))
-  = lemma_modulo r q b;
-    lemma_modulo r' q' b
-
-//TMP#reset-options
+let lemma_little_endian_is_injective_1 b q r q' r' =
+  lemma_mod_plus r q b;
+  lemma_mod_plus r' q' b;
+  lemma_mod_injective b r r'
 
 val lemma_little_endian_is_injective_2: b:word -> len:pos{len <= Seq.length b} -> Lemma
-  (requires (True))
-  (ensures  (
-    let s = Seq.slice b (Seq.length b - len) (Seq.length b) in
-    let s' = Seq.slice s 1 (Seq.length s) in
-    let s'' = Seq.slice b (Seq.length b - (len - 1)) (Seq.length b) in
-    s'' == s'))
+  (let s = Seq.slice b (Seq.length b - len) (Seq.length b) in
+   let s' = Seq.slice s 1 (Seq.length s) in
+   let s'' = Seq.slice b (Seq.length b - (len - 1)) (Seq.length b) in
+   s'' == s')
 let lemma_little_endian_is_injective_2 b len =
   let s = Seq.slice b (Seq.length b - len) (Seq.length b) in
   let s' = Seq.slice s 1 (Seq.length s) in
   let s'' = Seq.slice b (Seq.length b - (len - 1)) (Seq.length b) in
   Seq.lemma_eq_intro s' s''
 
-//TMP#reset-options "--initial_fuel 0 --max_fuel 0 --z3timeout 20"
-
-val lemma_little_endian_is_injective_3: b:word -> b':word  -> len:pos{len <= Seq.length b /\ len <= Seq.length b'} -> Lemma
-  (requires (Seq.slice b (Seq.length b - (len - 1)) (Seq.length b) == Seq.slice b' (Seq.length b' - (len-1)) (Seq.length b')
-    /\ Seq.index b (Seq.length b - len) = Seq.index b' (Seq.length b' - len)))
-  (ensures  (Seq.slice b (Seq.length b - len) (Seq.length b) == Seq.slice b' (Seq.length b' - len) (Seq.length b')))
+val lemma_little_endian_is_injective_3: b:word -> b':word -> len:pos{len <= Seq.length b /\ len <= Seq.length b'} -> Lemma
+  (requires (Seq.slice b (Seq.length b - (len - 1)) (Seq.length b) ==
+             Seq.slice b' (Seq.length b' - (len-1)) (Seq.length b')
+           /\ Seq.index b (Seq.length b - len) = Seq.index b' (Seq.length b' - len)))
+  (ensures  (Seq.slice b (Seq.length b - len) (Seq.length b) ==
+             Seq.slice b' (Seq.length b' - len) (Seq.length b')))
 let lemma_little_endian_is_injective_3 b b' len =
   Seq.lemma_eq_intro (Seq.slice b' (Seq.length b' - len) (Seq.length b'))
 		     (Seq.append (Seq.create 1 (Seq.index b' (Seq.length b' - len))) (Seq.slice b' (Seq.length b' - (len-1)) (Seq.length b')));
   Seq.lemma_eq_intro (Seq.slice b (Seq.length b - len) (Seq.length b))
 		     (Seq.append (Seq.create 1 (Seq.index b (Seq.length b - len))) (Seq.slice b (Seq.length b - (len-1)) (Seq.length b)))
 
-#reset-options "--initial_fuel 1 --max_fuel 1 --z3timeout 50"
-
 val lemma_little_endian_is_injective: b:word -> b':word ->
   len:nat{Seq.length b >= len /\ Seq.length b' >= len} -> Lemma
-    (requires (little_endian (Seq.slice b (Seq.length b - len) (Seq.length b))
-      = little_endian (Seq.slice b' (Seq.length b' - len) (Seq.length b')) ))
-    (ensures  (Seq.slice b (Seq.length b - len) (Seq.length b)
-	      == Seq.slice b' (Seq.length b' - len) (Seq.length b')))
+  (requires (little_endian (Seq.slice b (Seq.length b - len) (Seq.length b)) =
+             little_endian (Seq.slice b' (Seq.length b' - len) (Seq.length b')) ))
+  (ensures  (Seq.slice b (Seq.length b - len) (Seq.length b) ==
+             Seq.slice b' (Seq.length b' - len) (Seq.length b')))
 let rec lemma_little_endian_is_injective b b' len =
-  if len = 0 then (
+  if len = 0 then
     Seq.lemma_eq_intro (Seq.slice b (Seq.length b - len) (Seq.length b))
 		       (Seq.slice b' (Seq.length b' - len) (Seq.length b'))
-  )
-  else (
+  else
+    begin
     let s = Seq.slice b (Seq.length b - len) (Seq.length b) in
     let s' = Seq.slice b' (Seq.length b' - len) (Seq.length b') in
     assert(Seq.length s = len /\ Seq.length s' = len);
@@ -180,24 +201,68 @@ let rec lemma_little_endian_is_injective b b' len =
     lemma_little_endian_is_injective_2 b' len;
     lemma_little_endian_is_injective b b' (len - 1);
     lemma_little_endian_is_injective_3 b b' len
-  )
+    end
+
+val lemma_pad_0_injective: b0:Seq.seq UInt8.t -> b1:Seq.seq UInt8.t -> l:nat -> Lemma
+  (requires (pad_0 b0 l == pad_0 b1 l))
+  (ensures  (b0 == b1))
+let lemma_pad_0_injective b0 b1 l =
+  SeqProperties.lemma_append_inj b0 (Seq.create l 0uy) b1 (Seq.create l 0uy);
+  Seq.lemma_eq_intro b0 b1
+
+val lemma_encode_16_injective: w0:word_16 -> w1:word_16 -> Lemma
+  (requires (encode_16 w0 == encode_16 w1))
+  (ensures (w0 == w1))
+let lemma_encode_16_injective w0 w1 =
+  lemma_little_endian_lt_2_128 w0;
+  lemma_little_endian_lt_2_128 w1;
+  lemma_mod_plus_injective p_1305 (pow2 128) (little_endian w0) (little_endian w1);
+  assert (little_endian w0 == little_endian w1);
+  Seq.lemma_eq_intro (Seq.slice w0 0 16) w0;
+  Seq.lemma_eq_intro (Seq.slice w1 0 16) w1;
+  lemma_little_endian_is_injective w0 w1 16
+
+#reset-options "--initial_fuel 1 --max_fuel 1 --initial_ifuel 0 --max_ifuel 0"
+
+val lemma_encode_pad_injective: p0:Seq.seq elem -> t0:Seq.seq UInt8.t -> p1:Seq.seq elem -> t1:Seq.seq UInt8.t -> Lemma
+  (requires
+     Seq.length t0 == Seq.length t1 /\
+     encode_pad p0 t0 == encode_pad p1 t1)
+  (ensures p0 == p1 /\ t0 == t1)
+  (decreases (Seq.length t0))
+let rec lemma_encode_pad_injective p0 t0 p1 t1 =
+  let l = Seq.length t0 in
+  if l = 0 then Seq.lemma_eq_intro t0 t1
+  else if l < 16 then
+    begin
+    let w0 = pad_0 t0 (16 - l) in
+    let w1 = pad_0 t1 (16 - l) in
+    SeqProperties.lemma_append_inj
+      p0 (Seq.create 1 (encode_16 w0))
+      p1 (Seq.create 1 (encode_16 w1));
+    lemma_index_create 1 (encode_16 w0) 0;
+    lemma_index_create 1 (encode_16 w1) 0;
+    lemma_encode_16_injective w0 w1;
+    lemma_pad_0_injective t0 t1 (16 -l)
+    end
+  else
+    let w0, t0' = SeqProperties.split_eq t0 16 in
+    let w1, t1' = SeqProperties.split_eq t1 16 in
+    let p0' = SeqProperties.snoc p0 (encode_16 w0) in
+    let p1' = SeqProperties.snoc p1 (encode_16 w1) in
+    assert (encode_pad p0' t0' == encode_pad p1' t1');
+    lemma_encode_pad_injective p0' t0' p1' t1';
+    SeqProperties.lemma_append_inj
+      p0 (Seq.create 1 (encode_16 w0))
+      p1 (Seq.create 1 (encode_16 w1));
+    lemma_index_create 1 (encode_16 w0) 0;
+    lemma_index_create 1 (encode_16 w1) 0;
+    lemma_encode_16_injective w0 w1
 
 
 (* * *********************************************)
 (* *        Poly1305 functional invariant        *)
 (* * *********************************************)
-
-#reset-options "--initial_fuel 4 --max_fuel 4"
-
-let lemma_prime_is_greater_than_2_128 (u:unit) : Lemma
-  (requires True)
-  (ensures  (p_1305 > pow2 128))
-  = cut (pow2 3 = 8);
-    Math.Lib.pow2_increases_lemma 130 129;
-    Math.Lib.pow2_increases_lemma 129 128;
-    Math.Lib.pow2_increases_lemma 128 3
-
-//TMP#reset-options
 
 let seq_head (vs:seq 'a {Seq.length vs > 0}) = Seq.slice vs 0 (Seq.length vs - 1)
 
@@ -221,6 +286,5 @@ let clamp r =
   let r = fix r  8 252uy in 
   let r = fix r 12 252uy in 
   little_endian r
-
 
 let mac_1305 (vs:seq elem) r s = (trunc_1305 (poly vs r) + little_endian s) % pow2 128
