examples/low-level/crypto/Math.Lemmas.fst
@@ -3,17 +3,13 @@ module Math.Lemmas
 open FStar.Mul
 open Math.Axioms
 
-(** Usefull lemmas for future proofs **)
-val modulo_lemma_0: a:nat -> b:pos -> Lemma (requires (a < b)) (ensures (a % b = a))
-let modulo_lemma_0 a b = ()
-
-(* Lemma: definition of the euclidian division for nats *)
-val euclidian_div_axiom:
+(* Lemma: definition of the euclidean division for nats *)
+val euclidean_div_axiom:
   a:nat -> b:pos ->
   Lemma
     (requires (True))
     (ensures ( a - b * (a / b) >= 0 /\ a - b * (a / b) < b ))
-let euclidian_div_axiom a b = ()
+let euclidean_div_axiom a b = ()
 
 (* Lemma: multiplication is right distributive over addition *)
 val distributivity_add_left:
@@ -231,14 +227,14 @@ val mul_incr : a:nat -> b:nat -> c:nat ->
 		       (ensures ( a * b <= a * c /\ b * a <= c * a))
 let mul_incr a b c = ()
 
-(* Lemma : loss of precision in euclidian division *)
+(* Lemma : loss of precision in euclidean division *)
 val multiply_fractions:
   a:nat -> n:pos ->
   Lemma
     (requires (True))
     (ensures ( n * ( a / n ) <= a ))
 let multiply_fractions a n =
-  (euclidian_div_axiom a n)
+  (euclidean_div_axiom a n)
 
 (* Lemma : distributivity of minus over parenthesized sum *)
 val paren_sub: a:int -> b:int -> c:int -> Lemma ((a - (b + c) = a - b - c /\ a - (b - c) = a - b + c))
@@ -255,3 +251,81 @@ let nat_plus_nat_is_nat n m = ()
 
 val modulo_lemma: a:nat -> b:pos -> Lemma (requires (a < b)) (ensures (a % b = a))
 let modulo_lemma a b = ()
+
+#set-options "--initial_fuel 0 --max_fuel 0 --initial_ifuel 0 --max_ifuel 0"
+
+val lemma_div_mod: a:nat -> p:pos -> Lemma (a = p * (a / p) + a % p)
+let lemma_div_mod a p = ()
+
+val lemma_mod_lt: a:int -> p:pos -> Lemma (0 <= a % p /\ a % p < p)
+let lemma_mod_lt a p = ()
+
+val lemma_eq_trans_2: w:int -> x:int -> y:int -> z:int ->
+  Lemma
+  (requires (w = x /\ x = y /\ y = z))
+  (ensures  (x = z))
+let lemma_eq_trans_2 w x y z = ()
+
+val lemma_mod_plus: a:nat -> b:nat -> p:pos ->
+  Lemma ((a + b * p) % p = a % p)
+let lemma_mod_plus a b p =
+  lemma_div_mod a p;
+  lemma_div_mod (a + b * p) p;
+  lemma_mod_lt a p;
+  lemma_mod_lt (a + b * p) p;
+  assert ((a + b * p) % p - a % p = p * (b + a / p - (a + b * p) / p));
+  assert ((a + b * p) % p = a + b * p - p * ((a + b * p) / p));
+  assert (a % p = a - p * (a / p));
+  assert (a + b * p - p * ((a + b * p) / p) = a - p * (a / p));
+  let w = (a + b * p) % p in
+  let x = a + b * p - p * ((a + b * p) / p) in
+  let z = a % p in
+  let y = a - p * (a / p) in
+  lemma_eq_trans_2 w x y z
+
+val lemma_mod_injective: p:pos -> a:nat -> b:nat ->
+  Lemma
+  (requires (a < p /\ b < p /\ a % p = b % p))
+  (ensures  (a = b))
+let lemma_mod_injective p a b = ()
+
+val lemma_mul_sub_distr: a:int -> b:int -> c:int ->
+  Lemma (a * b - a * c = a * (b - c))
+let lemma_mul_sub_distr a b c = ()
+
+val lemma_div_exact: a:nat -> p:pos ->
+  Lemma
+  (requires (a % p = 0))
+  (ensures  (a = p * (a / p)))
+let lemma_div_exact a p = ()
+
+val lemma_mod_spec: a:nat -> p:pos ->
+  Lemma (a / p = (a - (a % p)) / p)
+let lemma_mod_spec a p =
+  lemma_div_mod a p;
+  assert (a = p * (a / p) + a % p);
+  assert (a % p = a - p * (a / p));
+  assert (a - (a % p) = p * (a / p));
+  lemma_mod_plus 0 (a / p) p;
+  assert ((p * (a / p)) % p = 0);
+  lemma_div_exact (p * (a / p)) p
+
+val lemma_mod_spec2: a:nat -> p:pos ->
+  Lemma (let q:nat = (a - (a % p)) / p in a = (a % p) + q * p)
+let lemma_mod_spec2 a p =
+  lemma_mod_spec a p
+
+val lemma_mod_plus_injective: p:pos -> a:nat -> b:nat -> c:nat ->
+  Lemma
+  (requires (b < p /\ c < p /\ (a + b) % p = (a + c) % p))
+  (ensures  (b = c))
+let lemma_mod_plus_injective p a b c =
+  lemma_mod_spec2 (a + b) p;
+  lemma_mod_spec2 (a + c) p;
+  let r = (a + b) % p in
+  let qb = ((a + b) - r) / p in
+  let qc = ((a + c) - r) / p in
+  assert (a + b = (a + c) + p * qb - p * qc);
+  lemma_mul_sub_distr p qb qc;
+  assert (b = c + p * (qb - qc));
+  assert (qb - qc = 0)
